Proven measure rule. Modifications in the logic and the semantics to fix an error in the paper semantics when the measuring is over all the variables of the heap.

QSemanticsBig.thy
@@ -1,5 +1,5 @@
 (* Title:     Quantum-Semantics/QSemantics.thy
-   Author:    David Sanan, Nanyang Technological University 
+   Author:    David Sanan, Nanyang Technological University m
    Copyright   2020
    License:     BSD
 *)
@@ -15,12 +15,77 @@ text \<open>Semantics for quantum programs\<close>
 (* m = partial_state2.ptensor_mat (dims_heap \<vv>) (q \<sigma>) ((Q_domain \<vv>)-(q \<sigma>)) (M::complex mat) (1\<^sub>m (card ((Q_domain \<vv>) - (q \<sigma>))))*)
 (* abbreviation "tensor_vec \<equiv> partial_state2.ptensor_vec" *)
 
-definition
+(* definition
   unit_vecl :: "nat \<Rightarrow> nat \<Rightarrow> complex list"
-  where "unit_vecl n i = list_of_vec (unit_vec n i)"
+  where "unit_vecl n i = list_of_vec (unit_vec n i)" *)
 
-definition Q_domain_var::"nat set \<Rightarrow> q_vars \<Rightarrow> nat set "
-  where "Q_domain_var q qvars \<equiv> \<Union> (qvars ` q)"
+
+
+definition aijv::"nat set \<Rightarrow> nat set \<Rightarrow> complex vec  \<Rightarrow> nat \<Rightarrow> nat \<Rightarrow>  complex"
+  where "aijv d1 d2 v i j\<equiv>  v$(partial_state2.pencode12 d1 d2 (i,j))"
+
+lemma eq_vec_aijv:
+      assumes a0:"i<(dim_vec v)" and a1:"dim_vec (v::complex vec) = (2^(card v1)) * (2^(card v2))" and
+              a2:"finite v1" and a3:"finite v2" and a4:"v1 \<inter> v2 = {}"        
+       shows "v $ i = aijv v1 v2 v 
+                    (partial_state.encode1 (list_dims (v1 \<union> v2))
+                       (partial_state2.vars1' v1 v2) i) 
+                    (partial_state.encode2 (list_dims (v1 \<union> v2)) 
+                       (partial_state2.vars1' v1 v2) i)"
+proof-
+  interpret ps2:partial_state2 "(replicate ((2^(card v1)) * (2^(card v2))) 2)" v1 v2
+    apply standard using a2 a3 a4  by auto
+  let ?i = "(\<lambda>i. partial_state.encode1 ps2.dims0 (partial_state2.vars1' v1 v2) i)"
+  let ?j = "(\<lambda>i. partial_state.encode2 ps2.dims0 (partial_state2.vars1' v1 v2) i)"
+   have "v $ i = aijv v1 v2 v (?i i) (?j i)"
+    unfolding aijv_def using a0
+    by (simp add: a1 card_Un_disjoint partial_state.encode12_inv power_add ps2.dims0_def 
+          ps2.disjoint ps2.finite_v1 
+        ps2.finite_v2 ps2.pencode12_def ps2.vars0_def state_sig.d_def)  
+  moreover have "ps2.dims0 = (list_dims (v1 \<union> v2))"
+    by (simp add: list_dims_def ps2.dims0_def ps2.vars0_def)
+  ultimately show ?thesis 
+    unfolding  list_dims_def ps2.dims0_def ps2.vars0_def  by auto
+qed
+
+lemma eq_vec_aijv_v2_empty:
+      assumes a0:"i<(dim_vec v)" and a1:"dim_vec (v::complex vec) = (2^(card v1)) * (2^(card v2))" and
+              a2:"finite v1" and a3:"v2 = {}" and a4:"v1 \<inter> v2 = {}"        
+       shows "v $ i = aijv v1 v2 v i 0"
+proof-
+  interpret ps2:partial_state2 "(replicate ((2^(card v1)) * (2^(card v2))) 2)" v1 v2
+    apply standard using a2 a3 a4  by auto
+  let ?i = "(\<lambda>i. partial_state.encode1 ps2.dims0 (partial_state2.vars1' v1 v2) i)"
+  let ?j = "(\<lambda>i. partial_state.encode2 ps2.dims0 (partial_state2.vars1' v1 v2) i)"
+  have "v $ i = aijv v1 v2 v (?i i) (?j i)"
+    unfolding aijv_def using a0
+    by (simp add: a1 card_Un_disjoint partial_state.encode12_inv power_add ps2.dims0_def 
+          ps2.disjoint ps2.finite_v1 
+        ps2.finite_v2 ps2.pencode12_def ps2.vars0_def state_sig.d_def)  
+  moreover have "(?j i) = 0" 
+    unfolding partial_state.encode2_def ps2.dims0_def    
+    using a3 digit_decode_non_vars1 partial_state.dims2_def 
+          partial_state2.vars1'_def ps2.partial_state2_axioms ps2.vars0_def 
+    by auto
+  moreover have "(?i i) = i" using a3
+    unfolding  list_dims_def ps2.dims0_def ps2.vars0_def apply auto
+    by (metis Int_absorb a0 digit_decode_vars ind_in_set_id length_replicate local.a1 order_refl partial_state.dims2_def partial_state.encode2_alter partial_state2.length_dims0_minus_vars2'_is_vars1' partial_state2.vars1'_def prod_list_replicate ps2.d0_def ps2.d1_def ps2.d2_def ps2.dims0_def ps2.dims1_def ps2.dims2_def ps2.dims_product ps2.finite_v1 ps2.nths_vars1' ps2.nths_vars1'_comp ps2.partial_state2_axioms ps2.ptensor_encode1_encode2 ps2.vars0_def sup_bot.right_neutral)   
+  ultimately show ?thesis using a3
+     by auto    
+qed
+
+definition vector_aij::"nat set \<Rightarrow> nat set \<Rightarrow> complex vec  \<Rightarrow> nat \<Rightarrow> complex vec"
+  where "vector_aij d1 d2 v i \<equiv> Matrix.vec (2^card d2) (\<lambda>j. aijv d1 d2 v i j)"
+
+definition list_aij::"nat set \<Rightarrow> nat set \<Rightarrow> complex vec  \<Rightarrow> nat \<Rightarrow> complex list"
+  where "list_aij d1 d2 v i \<equiv> map (\<lambda>j. aijv d1 d2 v i j) [0..<2^card d2]"
+
+definition aij ::"'s state \<Rightarrow> 's expr_q  \<Rightarrow> ('s, complex list) expr \<Rightarrow> nat \<Rightarrow> nat \<Rightarrow>complex" 
+  where "aij s q v i j \<equiv> let st = get_stack s ; qv = fst (get_qstate s); 
+                             vars = Q_domain qv; d1 = q st; d2 = vars - d1;
+                             vec = vec_of_list (v st) in 
+                             aijv d1 d2 vec i j"
+
 
 definition matrix_sep :: "nat set \<Rightarrow>  QStateM \<Rightarrow> complex mat \<Rightarrow>  QStateM" 
   where "matrix_sep heap_ind q M \<equiv>
@@ -32,21 +97,19 @@ definition matrix_sep :: "nat set \<Rightarrow>  QStateM \<Rightarrow> complex m
                                (M::complex mat) (1\<^sub>m (2^(card var_r)))  in 
              QStateM (QStateM_map q, QState (var_d, list_of_vec (m *\<^sub>v v)))"
 
-lemma "\<Union> (QStateM_map q ` hi) \<noteq> {} \<Longrightarrow> sep_vars = \<Union> ((QStateM_map q) ` hi) \<Longrightarrow>
-       var_d =  QStateM_vars q \<Longrightarrow> var_r = var_d - sep_vars \<Longrightarrow> v = QStateM_vector q \<Longrightarrow> 
-       QStateM_map (matrix_sep hi q M) = QStateM_map q \<and> 
-       QStateM_vars (matrix_sep hi q M) = QStateM_vars q \<and>
-       QStateM_list (matrix_sep hi q M) = 
-         list_of_vec (ptensor_mat sep_vars var_r
-                               (M::complex mat) (1\<^sub>m (2^(card var_r))) *\<^sub>v 
-                      QStateM_vector q)"  
-proof- 
+
+lemma matrix_sep_wf:
+      "\<Union> (QStateM_map q ` hi) \<noteq> {} \<Longrightarrow> sep_vars = \<Union> ((QStateM_map q) ` hi) \<Longrightarrow>
+       var_d =  QStateM_vars q \<Longrightarrow> var_r = var_d - sep_vars \<Longrightarrow> 
+       QStateM(m, QState(vs,v')) = matrix_sep hi q M \<Longrightarrow>
+       QState_wf (vs,v') \<and> QStateM_wf (m,QState(vs,v'))"
+proof-     
   assume a0:"\<Union> (QStateM_map q ` hi) \<noteq> {}" and
    a1:"sep_vars = \<Union> ((QStateM_map q) ` hi)" and
    a2:"var_d =  QStateM_vars q" and a3:"var_r = var_d - sep_vars" and
-   a4:"v = QStateM_vector q"
-
-  then have hi_not_e:"hi\<noteq>{}" by auto
+   
+   a5:"QStateM(m, QState(vs,v')) = matrix_sep hi q M"  
+  have hi_not_e:"hi\<noteq>{}" using a1 a0 by auto
   have "\<Union> (QStateM_map q ` hi) \<subseteq> Q_domain (QStateM_map q)"
     unfolding Q_domain_def
     by blast
@@ -72,9 +135,7 @@ proof-
     using finite_subset apply blast  
     using q_wf eq_QStateM_vars
     by (metis QState_rel3' finite_Diff)
-  have eq_domain_vars_map:"QStateM_vars q = {} \<Longrightarrow> 
-        Q_domain (QStateM_map q) = {}" 
-    apply auto unfolding qstate_def by (transfer, auto)  
+   
   have Q_wf:"QState_wf (QStateM_vars q, list_of_vec (?m *\<^sub>v ?v))"
     unfolding matrix_sep_def Let_def apply auto
     unfolding ps2.d0_def ps2.dims0_def ps2.vars0_def apply transfer   
@@ -88,13 +149,61 @@ proof-
     by blast   
   then have q:"QStateM_wf (QStateM_map q, QState (?var_d, list_of_vec (?m *\<^sub>v ?v)))"    
     using eq_QStateM_vars qm_wf by auto      
-  then show ?thesis unfolding matrix_sep_def Let_def 
-    using  f1 a1 a2 a3 a4
-    apply (auto simp add:  QStateM_wf_map QStateM_wf_vars )
-    using a1 a2 a3 a4 Q_wf q
-    by (metis QStateM_wf_list QState_list_idem q)
+  then have "m = QStateM_map q" using a5 unfolding matrix_sep_def Let_def 
+    using eq_QStateM_dest[OF  domain_map_not_e q] by metis
+  then show ?thesis using a5 unfolding matrix_sep_def Let_def 
+    using  eq_QStateM_dest[OF domain_map_not_e q]
+    by (smt QState.rep_eq QState_vars.rep_eq QState_vars_empty domain_map_not_e prod.collapse q)    
 qed
 
+lemma matrix_sep_dest:
+      "sep_vars \<noteq> {} \<Longrightarrow> sep_vars = Q_domain_var hi (QStateM_map q)  \<Longrightarrow>
+       var_d =  QStateM_vars q \<Longrightarrow> var_r = var_d - sep_vars \<Longrightarrow> 
+       QStateM_map (matrix_sep hi q M) = QStateM_map q \<and> 
+       QStateM_vars (matrix_sep hi q M) = QStateM_vars q \<and>
+       QStateM_list (matrix_sep hi q M) = 
+         list_of_vec (ptensor_mat sep_vars var_r
+                               (M::complex mat) (1\<^sub>m (2^(card var_r))) *\<^sub>v 
+                      QStateM_vector q)"  
+proof- 
+  assume a0:"sep_vars \<noteq> {}" and
+   a1:"sep_vars = Q_domain_var hi (QStateM_map q)" and
+   a2:"var_d =  QStateM_vars q" and a3:"var_r = var_d - sep_vars" 
+  note a1= a1[simplified Q_domain_var_def] and a0 = a0[simplified a1]
+  
+  then have hi_not_e:"hi\<noteq>{}" by auto
+  have "\<Union> (QStateM_map q ` hi) \<subseteq> Q_domain (QStateM_map q)"
+    unfolding Q_domain_def
+    by blast
+  then have domain_map_not_e:"Q_domain (QStateM_map q) \<noteq> {}"
+    using a0 hi_not_e apply transfer by auto  
+  let ?sep_vars = "\<Union> (QStateM_map q ` hi)" and
+      ?var_d = "QStateM_vars q" 
+  let ?var_r = "?var_d - ?sep_vars" and ?v = "QStateM_vector q" 
+  let ?m = "ptensor_mat ?sep_vars ?var_r M (1\<^sub>m (2 ^ card ?var_r))"  
+  obtain vs vas v' where 
+   matrix_sep_eq:"QStateM(vs, QState(vas,v')) = matrix_sep hi q M"
+    unfolding matrix_sep_def Let_def by auto
+  then have QState_wf:"QState_wf (vas,v')" and QStateM_wf:"QStateM_wf (vs,QState(vas,v'))"
+    using matrix_sep_wf[OF a0 a1 a2 a3  matrix_sep_eq]
+    by auto    
+  then have "QStateM_map (matrix_sep hi q M) = QStateM_map q"         
+    using  matrix_sep_eq
+    unfolding matrix_sep_def Let_def
+    by (metis QStateM_wf_map a0 matrix_sep_eq matrix_sep_wf)
+  moreover have "QStateM_vars (matrix_sep hi q M) = QStateM_vars q"
+    using matrix_sep_eq calculation
+    unfolding matrix_sep_def Let_def
+    by (metis QStateM_rel1 QStateM_vars.rep_eq qstate_def)
+  moreover have "QStateM_list (matrix_sep hi q M) = 
+         list_of_vec (ptensor_mat sep_vars var_r
+                               (M::complex mat) (1\<^sub>m (2^(card var_r))) *\<^sub>v 
+                      QStateM_vector q)"          
+    using matrix_sep_wf[OF a0 a1 a2 a3, of "QStateM_map q" ?var_d "list_of_vec (?m *\<^sub>v ?v)"]
+    unfolding matrix_sep_def Let_def
+    by (metis QStateM_wf_list QState_list_idem a3 local.a1 local.a2)
+  ultimately show ?thesis by auto
+qed
 
 (* definition matrix_sep :: "nat set \<Rightarrow> qstate \<Rightarrow> complex mat \<Rightarrow> qstate" 
   where "matrix_sep sep_vars q M \<equiv>
@@ -119,7 +228,7 @@ qed
     let qnprod = list_of_vec (((sqrt \<delta>k)::complex) \<cdot>\<^sub>v qn') in
        (\<delta>k, (fst q, QState (vars_dom, qnprod)))" *)
 
-definition measure_vars1::"nat \<Rightarrow>  nat set \<Rightarrow> qstate  \<Rightarrow> (real \<times> qstate)"
+(* definition measure_vars1::"nat \<Rightarrow>  nat set \<Rightarrow> qstate  \<Rightarrow> (real \<times> qstate)"
   where "measure_vars1 k  sep_vars q \<equiv>
    let qs = snd q in
    let vars_dom = QState_vars qs in
@@ -129,9 +238,9 @@ definition measure_vars1::"nat \<Rightarrow>  nat set \<Rightarrow> qstate  \<Ri
     let v' =  mk  *\<^sub>v v in 
     let \<delta>k =  Re ((vec_norm v')^2 div (vec_norm v)^2) in    
     let qnprod = list_of_vec (((sqrt \<delta>k)::complex) \<cdot>\<^sub>v v') in
-       (\<delta>k, (fst q, QState (vars_dom, qnprod)))" 
+       (\<delta>k, (fst q, QState (vars_dom, qnprod)))"  *)
 
-definition measure_vars::"nat \<Rightarrow>  nat set \<Rightarrow>  QStateM  \<Rightarrow> (real \<times>  QStateM)"
+(* definition measure_vars::"nat \<Rightarrow>  nat set \<Rightarrow>  QStateM  \<Rightarrow> (real \<times>  QStateM)"
   where "measure_vars k  sep_addr q \<equiv>
    let (qm, qs) = QStateM_unfold q in
    let vars_dom = QState_vars qs in
@@ -142,7 +251,1027 @@ definition measure_vars::"nat \<Rightarrow>  nat set \<Rightarrow>  QStateM  \<R
     let v' =  mk  *\<^sub>v v in 
     let \<delta>k =  Re ((vec_norm v')^2 div (vec_norm v)^2) in    
     let qnprod = list_of_vec (((sqrt \<delta>k)::complex) \<cdot>\<^sub>v v') in
-       (\<delta>k, QStateM(qm, QState (vars_dom, qnprod)))" 
+       (\<delta>k, QStateM(qm, QState (vars_dom, qnprod)))" *)
+
+definition measure_vars::"nat \<Rightarrow>  nat set \<Rightarrow>  QStateM  \<Rightarrow> (real \<times>  QStateM)"
+  where "measure_vars k  heap_ind q \<equiv>
+   let sep_vars = \<Union>((QStateM_map q) ` heap_ind) in
+   let Q' = matrix_sep heap_ind q (1\<^sub>k (2^(card sep_vars))) in
+   let \<delta>k =  Re ((vec_norm (QStateM_vector Q'))^2 div (vec_norm (QStateM_vector q))^2) in
+     (\<delta>k, (1 / sqrt (\<delta>k)) \<cdot>\<^sub>Q Q')"
+
+
+definition measure_vars'::"nat \<Rightarrow>  nat set \<Rightarrow>  QStateM  \<Rightarrow> (real \<times>  QStateM)"
+  where "measure_vars' k  heap_ind q \<equiv>   
+   let sep_vars = \<Union>((QStateM_map q) ` heap_ind) in  
+   let Q' = matrix_sep heap_ind q (1\<^sub>k (2^(card sep_vars))) in
+   let \<delta>k =  Re ((vec_norm (QStateM_vector Q'))^2 div (vec_norm (QStateM_vector q))^2) in   
+     if sep_vars = QStateM_vars q then 
+       (\<delta>k, QStateM (QStateM_map q, QState(QStateM_vars q, list_of_vec (unit_vec (2^(card sep_vars)) k))))
+     else (\<delta>k, (1 / sqrt (\<delta>k)) \<cdot>\<^sub>Q Q')"
+
+lemma measure_vars'_neq:"QStateM_vars Q \<noteq> \<Union>((QStateM_map Q) ` q) \<Longrightarrow> 
+      measure_vars' k q Q = measure_vars k q Q"
+  unfolding measure_vars'_def measure_vars_def Let_def by auto
+
+
+
+lemma eq_QState_dest: "vs \<noteq> {} \<Longrightarrow>
+       QState_wf (vs, v) \<Longrightarrow> 
+       QState(vs, v) = QState(vs', v') \<Longrightarrow> 
+       vs = vs' \<and> v = v'" 
+   apply transfer'
+  by (metis Pair_inject prod.collapse)
+
+lemma measure_vars_dest:
+  assumes 
+       a0:"n = Re ((vec_norm
+             (QStateM_vector
+               (matrix_sep q Q 1\<^sub>i (2 ^ card (\<Union> (QStateM_map Q ` q))))))\<^sup>2 /
+             (vec_norm (QStateM_vector Q))\<^sup>2)"
+     shows "measure_vars i q Q = (n, (1 / sqrt (n)) \<cdot>\<^sub>Q matrix_sep q Q (1\<^sub>i ((2::nat) ^ card (\<Union> (QStateM_map Q ` q)))))"
+  using a0
+  unfolding measure_vars_def Let_def by auto
+
+lemma measure_vars'_dest:  
+  assumes a0:"QStateM_vars Q = \<Union>((QStateM_map Q) ` q)" and 
+          a1:"n = Re ((vec_norm
+             (QStateM_vector
+               (matrix_sep q Q 1\<^sub>i (2 ^ card (\<Union> (QStateM_map Q ` q))))))\<^sup>2 /
+             (vec_norm (QStateM_vector Q))\<^sup>2)"
+  shows "measure_vars' i q Q = 
+       (n, QStateM (QStateM_map Q, QState(QStateM_vars Q, 
+           list_of_vec (unit_vec (2^(card (\<Union> (QStateM_map Q ` q)))) i))))"  
+  using a0 a1
+  unfolding measure_vars'_def Let_def by auto
+
+lemma measure_vars_wf:
+  assumes
+   a0:"(\<delta>k, QStateM(qm, QState (vars_dom, qnprod))) = measure_vars i q Q" and
+   a1:"\<forall>e \<in> q. QStateM_map Q e \<noteq> {}" and a2:"q \<noteq> {}" and a4:"\<delta>k > 0"
+  shows "QState_wf (vars_dom,qnprod) \<and> QStateM_wf (qm, QState(vars_dom,qnprod))"
+proof-
+  let ?sep_vars = "Q_domain_var q (QStateM_map Q)" 
+  let ?var_r = "(QStateM_vars Q) - ?sep_vars"
+  let ?m = "1\<^sub>i ((2::nat) ^ card ?sep_vars)"
+  let ?v = "matrix_sep q Q ?m"
+  let ?n = "((vec_norm
+             (QStateM_vector
+               (matrix_sep q Q 1\<^sub>i (2 ^ card ?sep_vars))))\<^sup>2 /
+             (vec_norm (QStateM_vector Q))\<^sup>2)"  
+  
+  have re_p_gt0:"Re ?n > 0"  and im_p_0:"Im ?n = 0"
+    using a0 a4 unfolding measure_vars_def Let_def vec_norm_def Q_domain_var_def by auto
+  then have QStateM_map_v:"QStateM_map ((1 / sqrt (Re ?n)) \<cdot>\<^sub>Q ?v) = QStateM_map ?v"
+    using sca_mult_qstatem_var_map by auto 
+
+  have qstate_eq:"qstate ((1 / sqrt (Re ?n)) \<cdot>\<^sub>Q ?v) = (1 / sqrt (Re ?n)) \<cdot>\<^sub>q qstate ?v"
+    using Im_complex_of_real Re_complex_of_real re_p_gt0 sca_mult_qstatem_var_qstate
+    by simp
+  have measure_eq:"QStateM(QStateM_map ?v, (1 / sqrt (Re ?n)) \<cdot>\<^sub>q qstate ?v) = 
+             QStateM(qm, QState (vars_dom, qnprod))"
+    using a0 unfolding sca_mult_qstatem_def measure_vars_def Let_def Q_domain_var_def  by auto
+    
+  have f1:"QStateM_wf (QStateM_map ?v, (1 / sqrt (Re ?n)) \<cdot>\<^sub>q qstate ?v) \<and> 
+           QState_wf (QState_vars ((1 / sqrt (Re ?n)) \<cdot>\<^sub>q qstate ?v), 
+                      QState_list ((1 / sqrt (Re ?n)) \<cdot>\<^sub>q qstate ?v))"    
+    by (metis qstate_eq QState_wf QStateM_wf QStateM_map_v) 
+  have "?sep_vars \<noteq> {}" unfolding Q_domain_var_def using a1 a2 by auto
+  then have qmap:"QStateM_map ?v = QStateM_map Q"     
+    by (auto simp add: matrix_sep_dest local.a1 local.a2)
+  have h1:"Q_domain (QStateM_map ?v) \<noteq> {}"
+    unfolding Q_domain_def
+    using local.a1 local.a2 qmap by auto
+  have "QStateM_map Q = qm" and eq_QState:"(1 / sqrt (Re ?n)) \<cdot>\<^sub>q qstate ?v = QState(vars_dom,qnprod)"
+    using eq_QStateM_dest[OF h1 conjunct1[OF f1] measure_eq] qmap  by auto  
+  then have QStateM_wf:"QStateM_wf (qm, QState(vars_dom,qnprod))"
+    using f1 qmap by auto 
+  
+  have "QState_vars ((1 / sqrt (Re ?n)) \<cdot>\<^sub>q qstate ?v) = vars_dom \<and>
+             QState_list ((1 / sqrt (Re ?n)) \<cdot>\<^sub>q qstate ?v) = qnprod"
+    using eq_QState_dest
+    by (metis QStateM_rel1 QState_refl QStateM_map_v qstate_eq eq_QState f1 local.h1)
+  moreover have "QState (vars_dom,qnprod) = (1 / sqrt (Re ?n)) \<cdot>\<^sub>q qstate ?v"
+    using eq_QState by auto
+  moreover have "QState_wf (QState_vars ((1 / sqrt (Re ?n)) \<cdot>\<^sub>q qstate ?v), QState_list ((1 / sqrt (Re ?n)) \<cdot>\<^sub>q qstate ?v))"
+    using f1
+    by auto
+  ultimately have "QState_wf (vars_dom, qnprod)" by auto
+  then show ?thesis using QStateM_wf by auto
+qed
+
+lemma measure_vars'_wf1:
+  assumes a0:"QStateM_vars Q = \<Union>((QStateM_map Q) ` q)" and
+   a1:"\<forall>e \<in> q. QStateM_map Q e \<noteq> {}" and a2:"q \<noteq> {}" and a4:"\<delta>k > 0"
+ shows "QState_wf (QStateM_vars Q,list_of_vec (unit_vec (2 ^ card (\<Union> (QStateM_map Q ` q))) i)) \<and> 
+        QStateM_wf (QStateM_map Q, QState(QStateM_vars Q,list_of_vec (unit_vec (2 ^ card (\<Union> (QStateM_map Q ` q))) i)))"
+proof-
+  have "QState_wf (QStateM_vars Q, QStateM_list Q)"
+    using QStateM_list.rep_eq QStateM_vars.rep_eq QState_wf by auto
+  then have "QState_wf (QStateM_vars Q,list_of_vec (unit_vec (2 ^ card (\<Union> (QStateM_map Q ` q))) i))"
+    using a0 a1 a2 by auto
+  moreover have "QStateM_wf (QStateM_map Q, QState(QStateM_vars Q,list_of_vec (unit_vec (2 ^ card (\<Union> (QStateM_map Q ` q))) i)))"
+    using a0 a1 a2 apply auto
+    using QStateM_wf QState_var_idem calculation eq_QStateM_vars apply auto[1]
+    using QState.rep_eq QStateM_wf QState_vars.rep_eq calculation eq_QStateM_vars apply auto[1]
+    using QStateM_wf by fastforce
+  ultimately show ?thesis by auto  
+qed
+
+lemma measure_vars'_wf:
+  assumes
+   a0:"(\<delta>k, QStateM(qm, QState (vars_dom, qnprod))) = measure_vars' i q Q" and
+   a1:"\<forall>e \<in> q. QStateM_map Q e \<noteq> {}" and a2:"q \<noteq> {}" and a4:"\<delta>k > 0"
+ shows "QState_wf (vars_dom,qnprod) \<and> QStateM_wf (qm, QState(vars_dom,qnprod))"
+proof-
+  let ?\<delta> = "Re ((vec_norm
+        (QStateM_vector (matrix_sep q Q 1\<^sub>i (2 ^ card (\<Union> (QStateM_map Q ` q))))))\<^sup>2 /
+      (vec_norm (QStateM_vector Q))\<^sup>2)" and 
+     ?v = " list_of_vec (unit_vec (2 ^ card (\<Union> (QStateM_map Q ` q))) i)"
+  { assume a00:"QStateM_vars Q = \<Union>((QStateM_map Q) ` q)"    
+    note measure = measure_vars'_dest[OF a00, of ?\<delta> i, simplified]  
+    
+    have QStateM_wf:"QStateM_wf (QStateM_map Q, QState (QStateM_vars Q, ?v))" and
+         QState_wf:"QState_wf (QStateM_vars Q,?v) "
+      using measure_vars'_wf1[OF a00 a1 a2 a4] by blast+      
+    
+    have q_domain:"Q_domain (QStateM_map Q) \<noteq> {}"
+      using Q_domain_def local.a1 local.a2 by auto        
+    then have vars_not_empty:"QStateM_vars Q \<noteq> {}"
+      using QStateM_rel1 QStateM_vars.rep_eq  qstate_def by auto
+    
+    have QStateM_eq:"QStateM (QStateM_map Q, QState (QStateM_vars Q, ?v)) =
+                   QStateM(qm, QState (vars_dom, qnprod))" using measure a0 by auto
+    
+    have eq_qm:"QStateM_map Q = qm"
+      using  measure q_domain QStateM_wf QStateM_eq
+      by (simp add: eq_QStateM_dest)                 
+    
+    have "QStateM_vars Q = vars_dom" 
+      using eq_QStateM_dest[OF q_domain QStateM_wf  QStateM_eq]
+      eq_QState_dest[OF vars_not_empty QState_wf] by blast
+    moreover have "?v = qnprod"   
+      using eq_QStateM_dest[OF q_domain QStateM_wf  QStateM_eq]
+      eq_QState_dest[OF vars_not_empty QState_wf] by blast
+    ultimately have ?thesis
+      using eq_qm local.QStateM_wf local.QState_wf by blast
+  }
+  moreover {
+    assume a00:"QStateM_vars Q \<noteq> \<Union>((QStateM_map Q) ` q)"
+    have eq:"(\<delta>k, QStateM(qm, QState (vars_dom, qnprod))) = measure_vars i q Q" 
+      using measure_vars'_neq[OF a00] a0 by auto
+    note measure_vars_wf[OF eq a1 a2 a4] 
+    then have ?thesis by auto
+  } ultimately show ?thesis by fastforce
+qed
+
+
+lemma measure_vars_dest_QStateM:
+  assumes   
+   a1:"\<forall>e \<in> q. QStateM_map Q e \<noteq> {}" and a2:"q \<noteq> {}" and a4:"0 < n" and 
+   a3:"n = Re ((vec_norm
+             (QStateM_vector
+               (matrix_sep q Q 1\<^sub>i (2 ^ card (\<Union> (QStateM_map Q ` q))))))\<^sup>2 /
+             (vec_norm (QStateM_vector Q))\<^sup>2)"
+ shows "QStateM_map (snd (measure_vars i q Q)) = QStateM_map Q \<and> 
+        QStateM_vars (snd (measure_vars i q Q)) = QStateM_vars Q \<and>
+        QStateM_vector (snd (measure_vars i q Q)) = 
+        QStateM_vector ((1 / sqrt (n)) \<cdot>\<^sub>Q (matrix_sep q Q (1\<^sub>i ((2::nat) ^ card (\<Union> (QStateM_map Q ` q))))))"
+proof-
+  let ?sep_vars = "Q_domain_var q (QStateM_map Q)" 
+  let ?m = "1\<^sub>i ((2::nat) ^ card ?sep_vars)"
+  let ?v = "matrix_sep q Q ?m"  
+  let ?var_r = "(QStateM_vars Q) - ?sep_vars"
+  have m:"measure_vars i q Q = (n, (1 / sqrt (n)) \<cdot>\<^sub>Q matrix_sep q Q 1\<^sub>i (2 ^ card (\<Union> (QStateM_map Q ` q))))" 
+    using measure_vars_dest[OF a3] by auto
+  have "?sep_vars \<noteq> {}" unfolding Q_domain_var_def using a1 a2 by auto 
+  then have  maps:"QStateM_map ?v = QStateM_map Q" and 
+       vars:"QStateM_vars ?v = QStateM_vars Q" and
+       list:"QStateM_list ?v = 
+         list_of_vec (ptensor_mat ?sep_vars ?var_r
+                               ?m (1\<^sub>m (2^(card ?var_r))) *\<^sub>v 
+                      QStateM_vector Q) "    
+    by (auto simp add: matrix_sep_dest local.a1 local.a2)
+  then have "QStateM_map (snd (measure_vars i q Q)) = QStateM_map Q"
+    using a3 a4 m sca_mult_qstatem_var_map unfolding Q_domain_var_def by auto
+  moreover have "QStateM_vars (snd (measure_vars i q Q)) = QStateM_vars Q"
+    using a3 a4 m sca_mult_qstatem_var_map vars
+    by (metis QStateM_rel1 QStateM_vars.rep_eq calculation qstate_def)
+  moreover have  "QStateM_vector (snd (measure_vars i q Q)) = 
+                  QStateM_vector ((1 / sqrt (n)) \<cdot>\<^sub>Q (matrix_sep q Q (1\<^sub>i ((2::nat) ^ card (\<Union> (QStateM_map Q ` q))))))"
+    using a3 a4 m sca_mult_qstatem_var_map vars
+    by simp
+  ultimately show ?thesis by auto
+qed
+
+lemma measure_vars'_dest_QStateM:
+  assumes a0:"QStateM_vars Q = \<Union>((QStateM_map Q) ` q)"   and   
+   a1:"\<forall>e \<in> q. QStateM_map Q e \<noteq> {}" and a2:"q \<noteq> {}" and a4:"0 < n" and 
+   a3:"n = Re ((vec_norm
+             (QStateM_vector
+               (matrix_sep q Q 1\<^sub>i (2 ^ card (\<Union> (QStateM_map Q ` q))))))\<^sup>2 /
+             (vec_norm (QStateM_vector Q))\<^sup>2)"
+ shows "QStateM_map (snd (measure_vars' i q Q)) = QStateM_map Q \<and> 
+        QStateM_vars (snd (measure_vars' i q Q)) = QStateM_vars Q \<and>
+        QStateM_vector (snd (measure_vars' i q Q)) = unit_vec (2^(card (\<Union> (QStateM_map Q ` q)))) i"
+proof-
+  let ?sep_vars = "Q_domain_var q (QStateM_map Q)" 
+  let ?v = "unit_vec (2^(card (\<Union> (QStateM_map Q ` q)))) i"  
+  let ?var_r = "(QStateM_vars Q) - ?sep_vars"
+  note m = measure_vars'_dest[OF a0 a3] 
+  have "?sep_vars \<noteq> {}" unfolding Q_domain_var_def using a1 a2 by auto   
+  then have "QStateM_map (snd (measure_vars' i q Q)) = QStateM_map Q"
+    using a3 a4 m  unfolding Q_domain_var_def
+    by (smt One_nat_def QStateM_rel1 QStateM_rel2 QStateM_wf_map QState_rel3' 
+          QState_var_idem a0 card_0_eq eq_QStateM_vars fst_conv index_unit_vec(3) 
+          length_list_of_vec n_not_Suc_n nat_power_eq_Suc_0_iff numeral_2_eq_2 snd_conv)
+  moreover have "QStateM_vars (snd (measure_vars' i q Q)) = QStateM_vars Q"
+    using a3 a4 m 
+    by (metis QStateM_rel1 QStateM_vars.rep_eq calculation qstate_def)
+  moreover have  "QStateM_vector (snd (measure_vars' i q Q)) = ?v"
+    using a3 a4 m apply auto
+    by (smt One_nat_def QStateM_rel1 QStateM_rel2 QStateM_wf_list QState_list_idem QState_rel3' 
+            QState_var_idem Q_domain_var_def \<open>Q_domain_var q (QStateM_map Q) \<noteq> {}\<close> 
+            a0 card_0_eq eq_QStateM_vars fst_conv index_unit_vec(3) 
+           length_list_of_vec n_not_Suc_n nat_power_eq_Suc_0_iff 
+           numeral_2_eq_2 snd_conv vec_list vec_of_list_QStateM_list) 
+  ultimately show ?thesis by auto
+qed
+
+
+lemma proj1_kk:
+  "k < 2^(card sep_vars) \<Longrightarrow> (1\<^sub>k (2^(card sep_vars))) $$ (k,k) = 1"
+    unfolding projection1_def by auto
+
+lemma proj1_not_kk:
+ "n < 2^(card v) \<Longrightarrow> m < 2^(card v) \<Longrightarrow> n\<noteq>k \<or> m\<noteq>k \<Longrightarrow>
+    (1\<^sub>k (2^(card v))) $$ (n,m) = 0"
+  unfolding projection1_def by auto 
+
+lemma proj1_one:"n < 2^(card v) \<Longrightarrow> m < 2^(card v) \<Longrightarrow> 
+  (1\<^sub>k (2^(card v))) $$ (n,m) = 1 \<longleftrightarrow> n = k \<and> m = k"
+  unfolding projection1_def by auto
+
+lemma one_mat_one:
+  "n < 2^(card v) \<Longrightarrow>  1\<^sub>m (2^(card v)) $$ (n,n) = 1"
+  by auto
+
+lemma one_mat_zero:
+  "i < 2^(card v) \<Longrightarrow> j < 2^(card v) \<Longrightarrow> i\<noteq>j \<Longrightarrow>  1\<^sub>m (2^(card v)) $$ (i,j) = 0"
+  by auto
+  
+lemma i_less_union: 
+  assumes a0:"(i::nat) < 2 ^ card v1 * 2 ^ card v2" and
+    a1:"v1 \<inter> v2 = {}" and
+    a2:"finite v1" and
+    a3:"finite v2"
+  shows"i < 2 ^ card (v1 \<union> v2)"
+  using a0 a1 a2 a3
+  by (simp add: card_Un_disjoint power_add)
+
+lemma mat_extend_1k_zero1: 
+     assumes a0:"finite v1" and a1:"finite v2" and a2:"v1 \<inter> v2 = {}" and
+       a3:"i < (2^(card v1)) * (2^(card v2))" and
+       a4:"j < (2^(card v1)) * (2^(card v2))" and "k < (2^(card v1))" and "i\<noteq>j"
+       shows "ptensor_mat v1 v2 ((1\<^sub>k (2^(card v1)))) (1\<^sub>m (2^(card v2))) $$ (i,j) = 0"
+proof-
+  let ?m1 = "1\<^sub>k (2^(card v1))" and ?m2 = "1\<^sub>m (2^(card v2))" and ?d = "list_dims (v1 \<union> v2)"
+  let ?v = "partial_state2.vars1' v1 v2"
+  interpret ps2:partial_state2 "list_dims (v1 \<union> v2)" v1 v2
+    apply standard using a0 a1 a2 unfolding list_dims_def by auto
+  have "ps2.dims0 = ?d" unfolding ps2.dims0_def list_dims_def ps2.vars0_def by auto
+  moreover have "ps2.ptensor_mat ?m1 ?m2 $$ (i,j) = 
+        ?m1 $$ (partial_state.encode1 ps2.dims0 ?v i, partial_state.encode1 ps2.dims0 ?v j) * 
+        ?m2 $$ (partial_state.encode2 ps2.dims0 ?v i, partial_state.encode2 ps2.dims0 ?v j)"
+    unfolding ps2.ptensor_mat_def 
+    apply (rule  partial_state.tensor_mat_eval, auto simp add: ps2.dims0_def state_sig.d_def ps2.vars0_def) 
+    using i_less_union[OF _ a2 a0 a1] a3 a4 by auto
+  ultimately show ?thesis
+    by (smt a3 a4 assms(7) length_replicate mult_not_zero one_mat_zero 
+            partial_state.d1_def partial_state.dims1_def 
+            partial_state.encode12_inv partial_state.encode1_lt 
+            power_add prod_list_replicate proj1_not_kk ps2.d_def 
+            ps2.dims0_def ps2.dims1_def ps2.dims2_def ps2.length_dims0 
+           ps2.nths_vars1' ps2.nths_vars2'_comp ps2.ptensor_encode2_encode1)
+qed
+
+lemma mat_extend_1k_zero2: 
+     assumes a0:"finite v1" and a1:"finite v2" and a2:"v1 \<inter> v2 = {}" and
+       a3:"i < (2^(card v1)) * (2^(card v2))" and
+       a4:"j < (2^(card v1)) * (2^(card v2))" and a5:"k < (2^(card v1))" and a6:"i=j" and
+       a7:"partial_state.encode1 (list_dims (v1 \<union> v2)) (partial_state2.vars1' v1 v2) i\<noteq>k"
+     shows "ptensor_mat v1 v2 ((1\<^sub>k (2^(card v1)))) (1\<^sub>m (2^(card v2))) $$ (i,j) = 0"
+proof-
+  let ?m1 = "1\<^sub>k (2^(card v1))" and ?m2 = "1\<^sub>m (2^(card v2))" and ?d = "list_dims (v1 \<union> v2)"
+  let ?v = "partial_state2.vars1' v1 v2"
+  interpret ps2:partial_state2 "list_dims (v1 \<union> v2)" v1 v2
+    apply standard using a0 a1 a2 unfolding list_dims_def by auto
+  have eq:"ps2.dims0 = ?d" unfolding ps2.dims0_def list_dims_def ps2.vars0_def by auto
+  have "ps2.ptensor_mat ?m1 ?m2 $$ (i,j) = 
+        ?m1 $$ (partial_state.encode1 ps2.dims0 ?v i, partial_state.encode1 ps2.dims0 ?v j) * 
+        ?m2 $$ (partial_state.encode2 ps2.dims0 ?v i, partial_state.encode2 ps2.dims0 ?v j)"
+    unfolding ps2.ptensor_mat_def 
+    apply (rule  partial_state.tensor_mat_eval, auto simp add: ps2.dims0_def state_sig.d_def ps2.vars0_def) 
+    using i_less_union[OF _ a2 a0 a1] a3 a4 by auto
+  also have "?m1 $$ (partial_state.encode1 ps2.dims0 ?v i, partial_state.encode1 ps2.dims0 ?v j) = 0"         
+    using a4 a6 a7 eq  partial_state.encode1_lt  prod_list_replicate length_replicate
+          power_add ps2.length_dims0 ps2.nths_vars1'
+    unfolding partial_state.d1_def projection1_def ps2.dims0_def 
+              ps2.dims1_def partial_state.dims1_def
+    by (smt index_mat(1) prod.simps(2) ps2.d_def )
+  finally show ?thesis by auto
+qed
+
+lemma mat_extend_1k_zero: 
+     assumes a0:"finite v1" and a1:"finite v2" and a2:"v1 \<inter> v2 = {}" and
+       a3:"i < (2^(card v1)) * (2^(card v2))" and
+       a4:"j < (2^(card v1)) * (2^(card v2))" and a5:"k < (2^(card v1))" and
+       a7:"partial_state.encode1 (list_dims (v1 \<union> v2)) (partial_state2.vars1' v1 v2) i\<noteq>k"
+     shows "ptensor_mat v1 v2 ((1\<^sub>k (2^(card v1)))) (1\<^sub>m (2^(card v2))) $$ (i,j) = 0"
+  using mat_extend_1k_zero2[OF a0 a1 a2 a3 a4 a5 _ a7] mat_extend_1k_zero1[OF a0 a1 a2 a3 a4 a5]
+  by auto
+
+lemma mat_extend_1k_one:
+assumes a0:"finite v1" and a1:"finite v2" and a2:"v1 \<inter> v2 = {}" and
+       a3:"i < (2^(card v1)) * (2^(card v2))" and
+       a4:"j < (2^(card v1)) * (2^(card v2))" and a5:"k < (2^(card v1))" and a6:"i=j" and
+       a7:"partial_state.encode1 (list_dims (v1 \<union> v2)) (partial_state2.vars1' v1 v2) i = k"
+     shows "ptensor_mat v1 v2 ((1\<^sub>k (2^(card v1)))) (1\<^sub>m (2^(card v2))) $$ (i,j) = 1"
+proof-
+  let ?m1 = "1\<^sub>k (2^(card v1))" and ?m2 = "1\<^sub>m (2^(card v2))" and ?d = "list_dims (v1 \<union> v2)"
+  let ?v = "partial_state2.vars1' v1 v2"
+  interpret ps2:partial_state2 "list_dims (v1 \<union> v2)" v1 v2
+    apply standard using a0 a1 a2 unfolding list_dims_def by auto
+  have eq:"ps2.dims0 = ?d" unfolding ps2.dims0_def list_dims_def ps2.vars0_def by auto
+  have "ps2.ptensor_mat ?m1 ?m2 $$ (i,j) = 
+        ?m1 $$ (partial_state.encode1 ps2.dims0 ?v i, partial_state.encode1 ps2.dims0 ?v j) * 
+        ?m2 $$ (partial_state.encode2 ps2.dims0 ?v i, partial_state.encode2 ps2.dims0 ?v j)"
+    unfolding ps2.ptensor_mat_def 
+    apply (rule  partial_state.tensor_mat_eval, auto simp add: ps2.dims0_def state_sig.d_def ps2.vars0_def) 
+    using i_less_union[OF _ a2 a0 a1] a3 a4 by auto
+  also have "?m1 $$ (partial_state.encode1 ps2.dims0 ?v i, partial_state.encode1 ps2.dims0 ?v j) = 1"
+    using a7 a6 a5
+    by (simp add: eq proj1_one)
+  also have  "?m2 $$ (partial_state.encode2 ps2.dims0 ?v i, partial_state.encode2 ps2.dims0 ?v j) = 1"
+    by (metis a4 a6 eq length_replicate list_dims_def one_mat_one 
+              partial_state.d1_def partial_state.dims1_def 
+              partial_state.encode1_lt power_add prod_list_replicate 
+              ps2.dims2_def ps2.length_dims0 ps2.nths_vars2'_comp 
+               ps2.ptensor_encode2_encode1 state_sig.d_def)    
+  finally show ?thesis by auto
+qed
+
+
+lemma row_i_not_k_zero:
+  assumes a0:"finite v1" and a1:"finite v2" and a2:"v1 \<inter> v2 = {}" and
+       a3:"i < (2^(card v1)) * (2^(card v2))" and
+       a4:"j < (2^(card v1)) * (2^(card v2))" and a5:"k < (2^(card v1))" and
+       a7:"partial_state.encode1 (list_dims (v1 \<union> v2)) (partial_state2.vars1' v1 v2) i \<noteq> k"  
+     shows "row (ptensor_mat v1 v2 ((1\<^sub>k (2^(card v1)))) (1\<^sub>m (2^(card v2))))  i $ j = 0"
+proof-
+  have "i < dim_col (ptensor_mat v1 v2 ((1\<^sub>k (2^(card v1)))) (1\<^sub>m (2^(card v2))))"    
+    using a3
+    by (simp add: ptensor_mat_dim_col[OF a0 a1 a2, of "(1\<^sub>k (2^(card v1)))" "1\<^sub>m (2^(card v2))"])       
+  moreover have " j < dim_col (ptensor_mat v1 v2 ((1\<^sub>k (2^(card v1)))) (1\<^sub>m (2^(card v2))))"
+    using a4
+    by (simp add: ptensor_mat_dim_col[OF a0 a1 a2, of "(1\<^sub>k (2^(card v1)))" "1\<^sub>m (2^(card v2))"])
+  ultimately have "row (ptensor_mat v1 v2 ((1\<^sub>k (2^(card v1)))) (1\<^sub>m (2^(card v2))))  i $ j = 
+        ptensor_mat v1 v2 ((1\<^sub>k (2^(card v1)))) (1\<^sub>m (2^(card v2)))$$(i,j)"          
+    unfolding row_def
+    apply (subst index_vec)
+    by auto  
+  then show ?thesis using mat_extend_1k_zero[OF a0 a1 a2 a3 a4 a5 a7]
+    by metis    
+qed
+
+
+lemma row_i_k_one:
+  assumes a0:"finite v1" and a1:"finite v2" and a2:"v1 \<inter> v2 = {}" and
+       a3:"i < (2^(card v1)) * (2^(card v2))" and
+       a4:"j < (2^(card v1)) * (2^(card v2))" and a5:"k < (2^(card v1))" and a6:"i=j" and
+       a7:"partial_state.encode1 (list_dims (v1 \<union> v2)) (partial_state2.vars1' v1 v2) i = k"  
+     shows "row (ptensor_mat v1 v2 ((1\<^sub>k (2^(card v1)))) (1\<^sub>m (2^(card v2))))  i $ j = 1"
+proof-
+  have "i < dim_col (ptensor_mat v1 v2 ((1\<^sub>k (2^(card v1)))) (1\<^sub>m (2^(card v2))))"    
+    using a3
+    by (simp add: ptensor_mat_dim_col[OF a0 a1 a2, of "(1\<^sub>k (2^(card v1)))" "1\<^sub>m (2^(card v2))"])       
+  moreover have " j < dim_col (ptensor_mat v1 v2 ((1\<^sub>k (2^(card v1)))) (1\<^sub>m (2^(card v2))))"
+    using a4
+    by (simp add: ptensor_mat_dim_col[OF a0 a1 a2, of "(1\<^sub>k (2^(card v1)))" "1\<^sub>m (2^(card v2))"])
+  ultimately have "row (ptensor_mat v1 v2 ((1\<^sub>k (2^(card v1)))) (1\<^sub>m (2^(card v2))))  i $ j = 
+        ptensor_mat v1 v2 ((1\<^sub>k (2^(card v1)))) (1\<^sub>m (2^(card v2)))$$(i,j)"          
+    unfolding row_def
+    apply (subst index_vec)
+    by auto
+  then show ?thesis 
+    using mat_extend_1k_one[OF a0 a1 a2 a3 a4 a5 a6 a7]
+    by metis    
+qed
+
+lemma row_i_k_zero:
+  assumes a0:"finite v1" and a1:"finite v2" and a2:"v1 \<inter> v2 = {}" and
+       a3:"i < (2^(card v1)) * (2^(card v2))" and
+       a4:"j < (2^(card v1)) * (2^(card v2))" and a5:"k < (2^(card v1))" and a6:"i\<noteq>j" and
+       a7:"partial_state.encode1 (list_dims (v1 \<union> v2)) (partial_state2.vars1' v1 v2) i = k"  
+     shows "row (ptensor_mat v1 v2 ((1\<^sub>k (2^(card v1)))) (1\<^sub>m (2^(card v2))))  i $ j = 0"
+proof-
+  have "i < dim_col (ptensor_mat v1 v2 ((1\<^sub>k (2^(card v1)))) (1\<^sub>m (2^(card v2))))"    
+    using a3
+    by (simp add: ptensor_mat_dim_col[OF a0 a1 a2, of "(1\<^sub>k (2^(card v1)))" "1\<^sub>m (2^(card v2))"])       
+  moreover have " j < dim_col (ptensor_mat v1 v2 ((1\<^sub>k (2^(card v1)))) (1\<^sub>m (2^(card v2))))"
+    using a4
+    by (simp add: ptensor_mat_dim_col[OF a0 a1 a2, of "(1\<^sub>k (2^(card v1)))" "1\<^sub>m (2^(card v2))"])
+  ultimately have "row (ptensor_mat v1 v2 ((1\<^sub>k (2^(card v1)))) (1\<^sub>m (2^(card v2))))  i $ j = 
+        ptensor_mat v1 v2 ((1\<^sub>k (2^(card v1)))) (1\<^sub>m (2^(card v2)))$$(i,j)"          
+    unfolding row_def
+    apply (subst index_vec)
+    by auto
+  then show ?thesis using mat_extend_1k_zero1[OF a0 a1 a2 a3 a4 a5 a6]
+    by metis    
+qed
+
+lemma row_ptensor_i_unit:
+  assumes a0:"finite v1" and a1:"finite v2" and a2:"v1 \<inter> v2 = {}" and      
+       a3:"i < (2^(card v1)) * (2^(card v2))" and
+       a5:"k < (2^(card v1))" and 
+       a7:"partial_state.encode1 (list_dims (v1 \<union> v2)) (partial_state2.vars1' v1 v2) i = k"
+     shows "row (ptensor_mat v1 v2 ((1\<^sub>k (2^(card v1)))) (1\<^sub>m (2^(card v2)))) i = 
+            unit_vec ((2^(card v1)) * (2^(card v2))) i"
+  apply rule
+  subgoal for j
+    using row_i_k_zero[OF a0 a1 a2 a3 _ a5, of j] row_i_k_one[OF a0 a1 a2 a3 _ a5, of j]
+    using a3 a7 by auto
+  by (simp add: a0 local.a1 local.a2 ptensor_mat_dim_col)  
+
+lemma row_ptensor_i_zero:
+  assumes a0:"finite v1" and a1:"finite v2" and a2:"v1 \<inter> v2 = {}" and      
+       a3:"i < (2^(card v1)) * (2^(card v2))" and
+       a5:"k < (2^(card v1))" and 
+       a7:"partial_state.encode1 (list_dims (v1 \<union> v2)) (partial_state2.vars1' v1 v2) i \<noteq> k"
+     shows "row (ptensor_mat v1 v2 ((1\<^sub>k (2^(card v1)))) (1\<^sub>m (2^(card v2)))) i = 
+            0\<^sub>v ((2^(card v1)) * (2^(card v2)))"
+  apply rule
+  subgoal for j
+    using row_i_not_k_zero[OF a0 a1 a2 a3 _ a5, of j]
+    using a3 a7 by auto
+  by (simp add: a0 local.a1 local.a2 ptensor_mat_dim_col)  
+
+
+lemma mat_product_vector_k:
+  assumes a0:"finite v1" and a1:"finite v2" and a2:"v1 \<inter> v2 = {}" and      
+       a3:"i < (2^(card v1)) * (2^(card v2))" and
+       a5:"k < (2^(card v1))" and 
+       a7:"partial_state.encode1 (list_dims (v1 \<union> v2)) (partial_state2.vars1' v1 v2) i = k" and
+       a8:"dim_vec v = (2^(card v1)) * (2^(card v2))"
+     shows "((ptensor_mat v1 v2 ((1\<^sub>k (2^(card v1)))) (1\<^sub>m (2^(card v2)))) *\<^sub>v v) $ i = v $ i"
+proof-
+  let ?m = "ptensor_mat v1 v2 ((1\<^sub>k (2^(card v1)))) (1\<^sub>m (2^(card v2)))"  
+  have a01:"(2 ^ card v1 * 2 ^ card v2) = dim_vec (?m *\<^sub>v v)"
+    by (simp add: a0 a3 local.a1 local.a2 ptensor_mat_dim_row)
+  have "i < (2 ^ card v1 * 2 ^ card v2)"
+    by (simp add: a0 a3 local.a1 local.a2 ptensor_mat_dim_row)
+  then show ?thesis using a01
+    apply auto
+    using scalar_prod_left_unit a8  
+    by (auto simp add: row_ptensor_i_unit[OF a0 a1 a2 a3 a5 a7] dest: carrier_vecI)
+qed
+
+lemma mat_product_vector_not_k:
+  assumes a0:"finite v1" and a1:"finite v2" and a2:"v1 \<inter> v2 = {}" and      
+       a3:"i < (2^(card v1)) * (2^(card v2))" and
+       a5:"k < (2^(card v1))" and 
+       a7:"partial_state.encode1 (list_dims (v1 \<union> v2)) (partial_state2.vars1' v1 v2) i \<noteq> k" and
+       a8:"dim_vec v = (2^(card v1)) * (2^(card v2))"
+     shows "((ptensor_mat v1 v2 ((1\<^sub>k (2^(card v1)))) (1\<^sub>m (2^(card v2)))) *\<^sub>v v) $ i = 0"
+proof-
+  let ?m = "ptensor_mat v1 v2 ((1\<^sub>k (2^(card v1)))) (1\<^sub>m (2^(card v2)))"  
+  have a01:"(2 ^ card v1 * 2 ^ card v2) = dim_vec (?m *\<^sub>v v)"
+    by (simp add: a0 a3 local.a1 local.a2 ptensor_mat_dim_row)
+  have "i < (2 ^ card v1 * 2 ^ card v2)"
+    by (simp add: a0 a3 local.a1 local.a2 ptensor_mat_dim_row)
+  then show ?thesis using a01
+    apply auto
+    using scalar_prod_left_unit a8  
+    by (auto simp add: row_ptensor_i_zero[OF a0 a1 a2 a3 a5 a7] dest: carrier_vecI)
+qed
+
+lemma v_scalar_mat_product_vector_not_k:
+  assumes a0:"finite v1" and a1:"finite v2" and a2:"v1 \<inter> v2 = {}" and      
+       a3:"i < (2^(card v1)) * (2^(card v2))" and
+       a5:"k < (2^(card v1))" and 
+       a7:"partial_state.encode1 (list_dims (v1 \<union> v2)) (partial_state2.vars1' v1 v2) i \<noteq> k" and
+       a8:"dim_vec v = (2^(card v1)) * (2^(card v2))"
+     shows "(a \<cdot>\<^sub>v ((ptensor_mat v1 v2 ((1\<^sub>k (2^(card v1)))) (1\<^sub>m (2^(card v2)))) *\<^sub>v v)) $ i = 0"
+  using mat_product_vector_not_k[OF a0 a1 a2 a3 a5 a7 a8]
+  by (simp add: a0 a3 local.a1 local.a2 ptensor_mat_dim_row) 
+
+lemma v_scalar_mat_product_vector_k:
+  assumes a0:"finite v1" and a1:"finite v2" and a2:"v1 \<inter> v2 = {}" and      
+       a3:"i < (2^(card v1)) * (2^(card v2))" and
+       a5:"k < (2^(card v1))" and 
+       a7:"partial_state.encode1 (list_dims (v1 \<union> v2)) (partial_state2.vars1' v1 v2) i = k" and
+       a8:"dim_vec v = (2^(card v1)) * (2^(card v2))"
+     shows "(a \<cdot>\<^sub>v ((ptensor_mat v1 v2 ((1\<^sub>k (2^(card v1)))) (1\<^sub>m (2^(card v2)))) *\<^sub>v v)) $ i = a * v $ i"
+  using mat_product_vector_k[OF a0 a1 a2 a3 a5 a7 a8]
+  by (simp add: a0 a3 local.a1 local.a2 ptensor_mat_dim_row) 
+
+lemma ptensor_unit_v_v_aij_not_k_zero:
+  assumes a0:"finite v1" and a1:"finite v2" and a2:"v1 \<inter> v2 = {}" and      
+       a3:"i < (2^(card v1)) * (2^(card v2))" and
+       a5:"k < (2^(card v1))" and 
+       a7:"partial_state.encode1 (list_dims (v1 \<union> v2)) (partial_state2.vars1' v1 v2) i \<noteq> k" and
+       a8:"dim_vec v = (2^(card v1)) * (2^(card v2))" 
+     shows "ptensor_vec v1 v2 (unit_vec (2 ^ card v1) k) (vector_aij v1 v2 v k) $ i = 0"
+proof-
+  let ?v1 = "unit_vec (2 ^ card v1) k" and ?v2 = "vector_aij v1 v2 v k"
+  interpret ps2:partial_state2 "replicate ((2^(card v1)) * (2^(card v2))) 2" "v1" "v2"
+    apply standard using a2 a1 a0 by auto
+  have "ptensor_vec v1 v2 (unit_vec (2 ^ card v1) k) (vector_aij v1 v2 v k) $ i = 
+        (?v1 $ (partial_state.encode1 (list_dims (v1 \<union> v2)) (partial_state2.vars1' v1 v2) i)) * 
+        (?v2 $ (partial_state.encode2  (list_dims (v1 \<union> v2)) (partial_state2.vars1' v1 v2) i))"
+    unfolding  ps2.ptensor_vec_def  ps2.dims0_def
+    by (simp add: a3 i_less_union list_dims_def local.a2 partial_state.tensor_vec_eval  
+                  ps2.finite_v1 ps2.finite_v2 ps2.vars0_def state_sig.d_def)
+  thus ?thesis
+    by (metis a3 a5 a7 i_less_union index_unit_vec(1) list_dims_def 
+         local.a2 mult_not_zero partial_state.d1_def partial_state.dims1_def 
+         partial_state.encode1_lt prod_list_replicate ps2.dims0_def ps2.dims1_def 
+         ps2.finite_v1 ps2.finite_v2 ps2.nths_vars1' ps2.vars0_def state_sig.d_def)  
+qed
+
+lemma ptensor_unit_v_v_aij_k_v_i:
+  assumes a0:"finite v1" and a1:"finite v2" and a2:"v1 \<inter> v2 = {}" and      
+       a3:"i < (2^(card v1)) * (2^(card v2))" and
+       a5:"k < (2^(card v1))" and 
+       a7:"partial_state.encode1 (list_dims (v1 \<union> v2)) (partial_state2.vars1' v1 v2) i = k" and
+       a8:"dim_vec v = (2^(card v1)) * (2^(card v2))" 
+     shows "ptensor_vec v1 v2 (unit_vec (2 ^ card v1) k) (vector_aij v1 v2 v k) $ i = v $ i"
+proof-
+  let ?v1 = "unit_vec (2 ^ card v1) k" and ?v2 = "vector_aij v1 v2 v k"
+  interpret ps2:partial_state2 "replicate ((2^(card v1)) * (2^(card v2))) 2" "v1" "v2"
+    apply standard using a2 a1 a0 by auto
+  have "ptensor_vec v1 v2 (unit_vec (2 ^ card v1) k) (vector_aij v1 v2 v k) $ i = 
+        (?v1 $ (partial_state.encode1 (list_dims (v1 \<union> v2)) (partial_state2.vars1' v1 v2) i)) * 
+        (?v2 $ (partial_state.encode2  (list_dims (v1 \<union> v2)) (partial_state2.vars1' v1 v2) i))"
+    unfolding  ps2.ptensor_vec_def  ps2.dims0_def
+    by (simp add: a3 i_less_union list_dims_def local.a2 partial_state.tensor_vec_eval  
+                  ps2.finite_v1 ps2.finite_v2 ps2.vars0_def state_sig.d_def)
+  moreover have "partial_state.encode2 (list_dims (v1 \<union> v2)) ps2.vars1' i < (2 ^ card v2)"
+    by (metis a3 i_less_union list_dims_def partial_state.d1_def partial_state.dims1_def 
+              partial_state.encode1_lt prod_list_replicate ps2.dims0_def 
+              ps2.dims2_def ps2.disjoint ps2.finite_v1 ps2.finite_v2 ps2.nths_vars2'_comp 
+              ps2.ptensor_encode2_encode1 ps2.vars0_def state_sig.d_def)    
+  then have "(?v2 $ (partial_state.encode2 (list_dims (v1 \<union> v2)) (partial_state2.vars1' v1 v2) i)) = 
+            v $ ps2.pencode12 (k, partial_state.encode2 (list_dims (v1 \<union> v2)) ps2.vars1' i) " 
+    unfolding vector_aij_def aijv_def using a7 a3  by auto        
+  then have "(?v2 $ (partial_state.encode2 (list_dims (v1 \<union> v2)) (partial_state2.vars1' v1 v2) i)) = v $ i"  
+    unfolding vector_aij_def aijv_def using a7 a3 apply auto
+    by (simp add:  i_less_union list_dims_def partial_state.encode12_inv 
+                  ps2.dims0_def ps2.disjoint ps2.finite_v1 ps2.finite_v2 
+                  ps2.pencode12_def ps2.vars0_def state_sig.d_def)    
+  moreover have "(?v1 $ (partial_state.encode1 (list_dims (v1 \<union> v2)) (partial_state2.vars1' v1 v2) i)) = 1"    
+    by (simp add: a7 a5)  
+  ultimately show ?thesis by auto  
+qed
+
+lemma mat_eq_ptensor_product_vector_i:
+  assumes a0:"finite v1" and a1:"finite v2" and a2:"v1 \<inter> v2 = {}" and      
+       a3:"(i::nat) < (2^(card v1)) * (2^(card v2))" and
+       a5:"k < (2^(card v1))" and
+       a8:"dim_vec v = (2^(card v1)) * (2^(card v2))" 
+     shows "(ptensor_mat v1 v2 (1\<^sub>k (2 ^ card v1)) (1\<^sub>m (2 ^ card v2)) *\<^sub>v v) $ i =
+            ptensor_vec v1 v2 (unit_vec (2 ^ card v1) k) (vector_aij v1 v2 v k) $ i"
+  using ptensor_unit_v_v_aij_k_v_i[OF a0 a1 a2 a3 a5 _ a8] 
+        ptensor_unit_v_v_aij_not_k_zero[OF a0 a1 a2 a3 a5 _ a8] 
+        mat_product_vector_not_k[OF a0 a1 a2 a3 a5 _ a8]  
+        mat_product_vector_k[OF a0 a1 a2 a3 a5 _ a8] 
+  by fastforce
+
+
+lemma mat_eq_ptensor_product_vector:
+  assumes a0:"finite v1" and a1:"finite v2" and a2:"v1 \<inter> v2 = {}" and             
+       a5:"k < (2^(card v1))" and
+       a8:"dim_vec v = (2^(card v1)) * (2^(card v2))"
+     shows "(ptensor_mat v1 v2 ((1\<^sub>k (2^(card v1)))) (1\<^sub>m (2^(card v2)))) *\<^sub>v v = 
+            ptensor_vec v1 v2 (unit_vec (2^(card v1)) k) (vector_aij v1 v2 v k)"
+proof-
+  let ?v = "(ptensor_mat v1 v2 ((1\<^sub>k (2^(card v1)))) (1\<^sub>m (2^(card v2)))) *\<^sub>v v"
+  let ?w = "ptensor_vec v1 v2 (unit_vec (2^(card v1)) k) (vector_aij v1 v2 v k)"
+  have "dim_vec ?v = dim_vec ?w"
+  proof- 
+    have "dim_vec ?v = (2^(card v1)) * (2^(card v2))"
+      by (simp add: a0 local.a1 local.a2 ptensor_mat_dim_row)
+    moreover have "dim_vec ?w = (2^(card v1)) * (2^(card v2))"   
+      by (metis a0  length_replicate local.a1 local.a2 nth_replicate
+                partial_state2.intro partial_state2.ptensor_mat_dim_col 
+               partial_state2.ptensor_vec_dim ptensor_mat_dim_col)
+    ultimately show ?thesis by auto
+  qed
+  moreover have "\<And>i. i < dim_vec ?w \<Longrightarrow> ?v $ i = ?w $ i"
+    using mat_eq_ptensor_product_vector_i[OF a0 a1 a2 _ a5 a8]
+    by (metis a0 calculation dim_mult_mat_vec local.a1 local.a2 ptensor_mat_dim_row)
+  ultimately show ?thesis by auto
+qed
+
+
+lemma v_scalar_mat_product_eq_ptensor:
+  assumes a0:"finite v1" and a1:"finite v2" and a2:"v1 \<inter> v2 = {}" and             
+       a5:"k < (2^(card v1))" and
+       a8:"dim_vec v = (2^(card v1)) * (2^(card v2))"
+     shows "a \<cdot>\<^sub>v ((ptensor_mat v1 v2 ((1\<^sub>k (2^(card v1)))) (1\<^sub>m (2^(card v2)))) *\<^sub>v v) = 
+            a \<cdot>\<^sub>v ptensor_vec v1 v2 (unit_vec (2^(card v1)) k) (vector_aij v1 v2 v k)"
+  using mat_eq_ptensor_product_vector[OF a0 a1 a2 a5 a8] by auto
+  
+
+
+
+lemma eq_sum_v_p_encode:
+assumes a0:"finite v1" and a1:"finite v2" and a2:"v1 \<inter> v2 = {}" and       
+       a3:"dim_vec (v::complex vec) = (2^(card v1)) * (2^(card v2))" 
+     shows "(\<Sum>i = 0..< (dim_vec v). (cmod (v $ i))\<^sup>2) = 
+           (\<Sum>i = 0 ..<2^(card v1). \<Sum>j = 0 ..<2^(card v2). (cmod (aijv v1 v2 v i j))\<^sup>2)"
+proof-
+  interpret ps2:
+    partial_state2 "replicate ((2^(card v1)) * (2^(card v2))) 2" "v1" "v2"
+    apply standard using a2 a1 a0 by auto
+  let ?i = "(\<lambda>i. partial_state.encode1 ps2.dims0 (partial_state2.vars1' v1 v2) i)"
+  let ?j = "(\<lambda>i. partial_state.encode2 ps2.dims0 (partial_state2.vars1' v1 v2) i)"
+  have "\<And>i. i<(dim_vec v) \<Longrightarrow>  
+              v $ i = aijv v1 v2 v (?i i) (?j i)"
+    unfolding aijv_def
+    by (simp add: a3 card_Un_disjoint partial_state.encode12_inv power_add ps2.dims0_def 
+          ps2.disjoint ps2.finite_v1 
+        ps2.finite_v2 ps2.pencode12_def ps2.vars0_def state_sig.d_def)
+  then have eq:"\<And>i. i<(dim_vec v) \<Longrightarrow>  
+              (cmod (v $ i))\<^sup>2 = (cmod (aijv v1 v2 v (?i i) (?j i)))\<^sup>2" by auto
+  have "(\<Sum>i = 0..< (dim_vec v). (cmod (v $ i))\<^sup>2) = 
+        (\<Sum>i = 0..< (dim_vec v). (cmod (v $ partial_state2.pencode12 v1 v2 (?i i,?j i)))\<^sup>2)"
+    using partial_state.encode12_inv ps2.dims_product 
+         ps2.partial_state2_axioms a3 partial_state2.pencode12_def 
+    unfolding  ps2.d0_def ps2.d1_def ps2.d2_def ps2.dims1_def ps2.dims2_def  state_sig.d_def by auto
+  also have "\<dots> = 
+             (\<Sum>i = 0 ..<2^(card v1). \<Sum>j = 0 ..<2^(card v2). (cmod (v $ partial_state2.pencode12 v1 v2 (i,j)))\<^sup>2)"    
+  proof-
+    have "dim_vec v = state_sig.d ps2.dims0" and
+         "partial_state.d2 ps2.dims0 ps2.vars1' = 2 ^ card v2" and
+         "partial_state.d1 ps2.dims0 ps2.vars1' = 2 ^ card v1"
+      using a3 unfolding state_sig.d_def
+      using ps2.d0_def ps2.d1_def ps2.dims0_def ps2.dims1_def 
+            ps2.dims2_def ps2.dims_product       
+      using partial_state.d2_def partial_state.dims2_def ps2.d2_def ps2.nths_vars2'
+      using partial_state.d1_def partial_state.dims1_def ps2.nths_vars1' by auto
+    thus ?thesis  
+      using partial_state.sum_encode[THEN sym, where dims1 = ps2.dims0 and vars1 = ps2.vars1']
+      by fastforce
+  qed       
+  finally show ?thesis unfolding aijv_def by auto
+qed
+  
+              
+lemma eq_v_aijv_i_j:  
+    assumes a0:"finite v1" and a1:"finite v2" and a2:"v1 \<inter> v2 = {}" and
+       a5:"k < (2^(card v1))" and
+       a8:"dim_vec v = (2^(card v1)) * (2^(card v2))"
+     shows "(vec_norm v)^2 = 
+            (\<Sum>i = 0 ..<2^(card v1). \<Sum>j = 0 ..<2^(card v2). (norm (aijv v1 v2 v i j))^2)"
+proof-
+  have " v \<bullet>c v = (\<Sum>i = 0 ..<dim_vec v. (v$i) * (conjugate (v$i)))"
+   unfolding scalar_prod_def by auto
+  also have "\<dots> =  (\<Sum>i = 0 ..<dim_vec v. (norm (v$i))\<^sup>2)"
+    using complex_norm_square conjugate_complex_def
+    by auto
+  also have " \<dots> = (\<Sum>i = 0 ..<2^(card v1). \<Sum>j = 0 ..<2^(card v2). (norm (aijv v1 v2 v i j))^2)"
+    using eq_sum_v_p_encode[OF a0 a1 a2 a8] by auto
+  finally have "v \<bullet>c v = (\<Sum>i = 0 ..<2^(card v1). \<Sum>j = 0 ..<2^(card v2). (norm (aijv v1 v2 v i j))^2)"
+    by auto
+  moreover have "(vec_norm v)^2 = v \<bullet>c v"
+    using power2_csqrt vec_norm_def by presburger
+  ultimately show ?thesis
+    by auto
+qed
+
+lemma 
+  assumes a0:"l \<noteq> k" and a1:"\<forall>i j. j < n \<and> i < m \<and> i \<noteq> k \<longrightarrow> f i j = 0" 
+  and a2:"l<m" 
+shows "(\<Sum>j = 0 ..<n. f l j) = 0"
+  using  a2 a0 a1
+  by simp
+
+lemma sum_f_i_lt_k_0:
+  assumes a0:"(m::nat) \<le> k" and a1:"\<forall>i j. j < n \<and> i < m \<and> i \<noteq> k \<longrightarrow> f i j = 0" and a2:"0<m"
+  shows "(\<Sum>i = 0 ..<m. \<Sum>j = 0 ..<n. f i j) = 0"
+  using a2 a1 a0
+proof(induct m rule:nat_induct_non_zero)
+  case 1
+  then show ?case by auto
+next
+  case (Suc m)
+  then have "(\<Sum>i = 0..<Suc m. sum (f i) {0..<n}) = 
+             (\<Sum>i = 0..< m. sum (f i) {0..<n}) + sum (f m) {0..<n} "
+    by auto
+  moreover have "sum (f m) {0..<n} = 0"
+    using Suc.prems(1) Suc.prems(2) by auto
+  moreover have "(\<Sum>i = 0..< m. sum (f i) {0..<n}) = 0"
+    by (metis Suc.hyps(2) Suc.prems(1) Suc.prems(2) Suc_eq_plus1 add_leD1 less_SucI)
+  ultimately show ?case by auto
+qed
+
+lemma sum_eq_sum_k_j:
+  assumes a0:"k < (m::nat)" and a1:"\<forall>i j. j < n \<and> i < m \<and> i \<noteq> k \<longrightarrow> f i j = 0" and a2:"0<m"
+  shows "(\<Sum>i = 0 ..<m. \<Sum>j = 0 ..<n. f i j) = (\<Sum>j = 0 ..<n. f k j)"
+
+  using a2 a0 a1 
+proof(induct m rule:nat_induct_non_zero)
+  case 1
+  then show ?case by auto
+next
+  case (Suc m)
+  then have sum_eq:"(\<Sum>i = 0..<Suc m. sum (f i) {0..<n}) = 
+             (\<Sum>i = 0..< m. sum (f i) {0..<n}) + sum (f m) {0..<n} "
+    by auto  
+  { assume a00:"k=m"        
+    then have "(\<Sum>i = 0..< m. sum (f i) {0..<n}) = 0"
+      using sum_f_i_lt_k_0[of m k n f]  a00 by (simp add: Suc.prems(2))
+    then have ?case using sum_eq a00 by auto
+  }
+  moreover { 
+    assume a00:"k\<noteq>m"    
+    then have ?case using sum_eq a00
+      using Suc.hyps(2) Suc.prems(1) Suc.prems(2) by auto 
+  }
+  ultimately show ?case by auto
+qed
+
+lemma  vec_norm_ptensor_eq_sum_norm_k:
+  assumes a0:"finite v1" and a1:"finite v2" and a2:"v1 \<inter> v2 = {}" and
+       a5:"k < (2^(card v1))" and
+       a8:"dim_vec v = (2^(card v1)) * (2^(card v2))"
+  shows "(vec_norm (((ptensor_mat v1 v2 ((1\<^sub>k (2^(card v1)))) (1\<^sub>m (2^(card v2)))) *\<^sub>v v)))^2  = 
+         (\<Sum>j = 0..<2^(card v2). norm (aijv v1 v2 v k j )^2)"
+proof-
+  interpret ps2:
+    partial_state2 "replicate ((2^(card v1)) * (2^(card v2))) 2" "v1" "v2"
+    apply standard using a2 a1 a0 by auto
+  let ?i = "(\<lambda>i. partial_state.encode1 ps2.dims0 (partial_state2.vars1' v1 v2) i)"
+  let ?j = "(\<lambda>i. partial_state.encode2 ps2.dims0 (partial_state2.vars1' v1 v2) i)"
+  let ?v = "(((ptensor_mat v1 v2 ((1\<^sub>k (2^(card v1)))) (1\<^sub>m (2^(card v2)))) *\<^sub>v v))"   
+  have dim_v:"dim_vec v = dim_vec ?v"
+    by (simp add: a8 ps2.d1_def ps2.d2_def ps2.dims1_def ps2.dims2_def ps2.dims_product)
+  then have "(vec_norm ?v)^2 = 
+            (\<Sum>i = 0 ..<2^(card v1). \<Sum>j = 0 ..<2^(card v2). (norm (aijv v1 v2 ?v i j))^2)"
+    using eq_v_aijv_i_j[OF a0 a1 a2 a5 a8[simplified dim_v]] by fastforce
+  also have "(\<Sum>i = 0 ..<2^(card v1). \<Sum>j = 0 ..<2^(card v2). (norm (aijv v1 v2 ?v i j))^2) = 
+             (\<Sum>j = 0..<2^(card v2). norm (aijv v1 v2 v k j )^2)"
+  proof-
+    have "\<And>i. i<(dim_vec ?v) \<Longrightarrow>  
+                 ?v $ i = aijv v1 v2 ?v (?i i) (?j i)"
+      unfolding aijv_def
+      by (simp add: partial_state.encode12_inv ps2.d0_def ps2.pencode12_def state_sig.d_def)
+    let ?f = "\<lambda>i j. (cmod (aijv v1 v2 ?v i j))\<^sup>2"
+    have "(\<Sum>i = 0..<2 ^ card v1.
+             \<Sum>j = 0..<2 ^ card v2.
+                (cmod (aijv v1 v2 ?v i j))\<^sup>2) =
+         (\<Sum>j = 0..<2 ^ card v2. (cmod (aijv v1 v2 ?v k j))\<^sup>2)"
+      apply (rule sum_eq_sum_k_j[of k "2 ^ card v1" "2 ^ card v2" ?f])
+      using a5 apply fastforce
+      unfolding aijv_def 
+      apply auto apply (rule  mat_product_vector_not_k[OF a0 a1 a2 _ _ _  a8])
+        apply (metis a8 dim_mult_mat_vec dim_v partial_state.d1_def 
+                     partial_state.d2_def partial_state.dims1_def 
+                     partial_state.dims2_def partial_state.encode12_lt 
+                     partial_state2.ptensor_mat_dim_row prod_list_replicate 
+                     ps2.d0_def ps2.dims1_def ps2.dims2_def 
+                     ps2.nths_vars1' ps2.nths_vars2' 
+                     ps2.partial_state2_axioms ps2.pencode12_def state_sig.d_def)
+      using a5 apply blast unfolding ps2.pencode12_def
+      by (metis list_dims_def partial_state.d1_def partial_state.d2_def 
+                partial_state.dims1_def partial_state.dims2_def 
+                partial_state.encode12_inv1 prod_list_replicate ps2.dims0_def 
+                ps2.dims1_def ps2.dims2_def ps2.nths_vars1' ps2.nths_vars2' ps2.vars0_def)          
+    also have "(\<Sum>j = 0..<2 ^ card v2. (cmod (aijv v1 v2 ?v k j))\<^sup>2) = 
+               (\<Sum>j = 0..<2 ^ card v2. (cmod (aijv v1 v2  v k j))\<^sup>2)"    
+    proof-
+      have "\<And>j. j < 2^card v2 \<Longrightarrow> (cmod (aijv v1 v2 ?v k j))\<^sup>2 = (cmod (aijv v1 v2 v k j))\<^sup>2"      
+        unfolding aijv_def using mat_product_vector_k[OF a0 a1 a2 _ _ _ a8]      
+        by (metis a5 list_dims_def partial_state.d1_def partial_state.d2_def
+                partial_state.dims1_def partial_state.dims2_def 
+                partial_state.encode12_inv1 partial_state.encode12_lt 
+                prod_list_replicate ps2.d0_def ps2.d1_def ps2.d2_def ps2.dims0_def 
+                ps2.dims1_def ps2.dims2_def ps2.dims_product ps2.nths_vars1' 
+                ps2.nths_vars2' ps2.pencode12_def ps2.vars0_def state_sig.d_def)                       
+      then show ?thesis by simp
+   qed         
+   finally show ?thesis by auto
+  qed
+  finally show ?thesis by auto
+qed
+
+lemma eq_norm: assumes a0:"finite v1" and a1:"finite v2" and a2:"v1 \<inter> v2 = {}" and             
+       a5:"k < (2^(card v1))" and
+       a8:"dim_vec v = (2^(card v1)) * (2^(card v2))"
+     shows "Re ((vec_norm (((ptensor_mat v1 v2 ((1\<^sub>k (2^(card v1)))) (1\<^sub>m (2^(card v2)))) *\<^sub>v v)))^2 
+                div (vec_norm v)^2) =
+            (\<Sum>j = 0..<2^(card v2). norm (aijv v1 v2 v k j )^2) / 
+             (\<Sum>i = 0 ..<2^(card v1). \<Sum>j = 0 ..<2^(card v2). norm (aijv v1 v2 v i j)^2 )"
+proof-
+  have "(vec_norm (((ptensor_mat v1 v2 ((1\<^sub>k (2^(card v1)))) (1\<^sub>m (2^(card v2)))) *\<^sub>v v)))^2 =
+        (\<Sum>j = 0..<2^(card v2). norm (aijv v1 v2 v k j )^2)"
+    using vec_norm_ptensor_eq_sum_norm_k[OF a0 a1 a2 a5 a8] by auto
+  moreover have "(vec_norm v)^2 = 
+                 (\<Sum>i = 0 ..<2^(card v1). 
+                    \<Sum>j = 0 ..<2^(card v2). norm (aijv v1 v2 v i j)^2 )"
+    using eq_v_aijv_i_j[OF a0 a1 a2 a5 a8] by auto
+  ultimately show ?thesis by auto
+qed
+
+lemma norm_v2_empty: assumes a0:"finite v1" and a1:"v2 = {}" and             
+       a5:"k < (2^(card v1))" and
+       a8:"dim_vec v = (2^(card v1)) * (2^(card v2))"
+     shows "Re ((vec_norm (((ptensor_mat v1 v2 ((1\<^sub>k (2^(card v1)))) (1\<^sub>m (2^(card v2)))) *\<^sub>v v)))^2 
+                div (vec_norm v)^2) =
+            (norm (v$k)^2) / (\<Sum>i = 0 ..<2^(card v1). norm (v$i)^2 )"
+proof-
+  have "Re ((vec_norm (((ptensor_mat v1 v2 ((1\<^sub>k (2^(card v1)))) (1\<^sub>m (2^(card v2)))) *\<^sub>v v)))^2 
+                div (vec_norm v)^2) = (\<Sum>j = 0..<2^(card v2). norm (aijv v1 v2 v k j )^2) / 
+             (\<Sum>i = 0 ..<2^(card v1). \<Sum>j = 0 ..<2^(card v2). norm (aijv v1 v2 v i j)^2 )"
+    using eq_norm[OF a0 _ _ a5 a8] using a1 by auto
+  moreover have "\<And>i. i <(2^(card v1)) \<Longrightarrow> aijv v1 v2 v k 0 = v $ k" using a1 unfolding aijv_def
+    using eq_vec_aijv_v2_empty
+    using a0 a5 a8 aijv_def by auto
+  moreover have "(\<Sum>j = 0..<2^(card v2). norm (aijv v1 v2 v k j )^2) =  norm (v$k)^2"
+    using a1 calculation(2)
+    by fastforce  
+  moreover have "(\<Sum>i = 0 ..<2^(card v1). \<Sum>j = 0 ..<2^(card v2). norm (aijv v1 v2 v i j)^2 )= 
+                 (\<Sum>i = 0 ..<2^(card v1). norm (v$i)^2)"
+    using a1 calculation(2)
+    by (metis (no_types) a0 a8 card_empty eq_sum_v_p_encode 
+            finite.emptyI inf_bot_right mult.right_neutral power.simps(1))    
+  ultimately show ?thesis by auto
+qed
+
+
+
+lemma  sqrt_norm_eq:
+   assumes a0:"finite v1" and a1:"v2 = {}" and             
+       a5:"k < (2^(card v1))" and
+       a8:"dim_vec v = (2^(card v1)) * (2^(card v2))" and 
+       a9:"\<delta>k = (norm (v$k))^2 / (\<Sum>i = 0 ..<2^(card v1). (norm (v$i))^2 )"
+     shows "sqrt \<delta>k = norm (v$k)  / sqrt (\<Sum>i = 0 ..<2^(card v1). norm (v$i)^2 )"
+proof-
+  have "\<And>a b. sqrt (a/b) = sqrt a / sqrt b"
+    using real_sqrt_divide by auto
+  moreover have "\<And>a. norm a \<ge> 0" by auto
+  then have "\<And>a. a\<ge>0 \<Longrightarrow> sqrt (a\<^sup>2) = a" by auto
+  ultimately show ?thesis using a9 by auto
+qed
+  
+lemma  vector_aij_v2_empty:
+  assumes a0:"finite v1" and a1:"v2 = {}" and             
+       a5:"k < (2^(card v1))" and
+       a8:"dim_vec v = (2^(card v1)) * (2^(card v2))" 
+     shows "vector_aij v1 v2 v k $ 0 = v$k"
+ unfolding vector_aij_def 
+ using eq_vec_aijv_v2_empty[OF _ a8 a0 a1 _] a5 a8 a1  by auto
+
+(*
+lemma  assumes a0:"finite v1" and a1:"v2 = {}" and             
+       a5:"k < (2^(card v1))" and
+       a8:"dim_vec v = (2^(card v1)) * (2^(card v2))" and 
+       a9:"\<delta>k = Re ((norm (v$k)^2) / (\<Sum>i = 0 ..<2^(card v1). norm (v$i)^2 ))" and 
+       a10:"(v'::complex vec) =(((1 / sqrt \<delta>k)\<cdot>\<^sub>v(vector_aij v1 v2 v k))) " 
+     shows "v' = ((\<Sum>i = 0 ..<2^(card v1). norm (v$i)^2))" *)
+
+lemma measure_vars_QStateM_map:
+  assumes           
+     a0:"(\<forall>e\<in>q. QStateM_map Q e \<noteq> {})" and a1:"q \<noteq> {}" and a2:"p>0" and
+     a3:"(p,Q') = measure_vars i q Q" 
+   shows "QStateM_map Q' = QStateM_map Q"
+     using measure_vars_dest_QStateM[OF a0 a1 a2]
+     by (metis a3 fst_conv measure_vars_dest snd_conv)
+
+lemma measure_vars'_QStateM_map:
+  assumes           
+     a0:"(\<forall>e\<in>q. QStateM_map Q e \<noteq> {})" and a1:"q \<noteq> {}" and a2:"p>0" and
+     a3:"(p,Q') = measure_vars' i q Q" 
+   shows "QStateM_map Q' = QStateM_map Q"
+  apply (cases "QStateM_vars Q = \<Union>((QStateM_map Q) ` q)")
+  using measure_vars'_dest_QStateM[OF _ a0 a1 a2]
+  apply (metis a3 fst_conv measure_vars'_dest snd_conv)
+  using measure_vars_dest_QStateM[OF a0 a1 a2]
+  by (metis (full_types) a0 a3 local.a1 local.a2 measure_vars'_neq measure_vars_QStateM_map)
+  
+lemma  measure_vars_eq_length_vector:
+  assumes
+   a0:"(\<delta>k, QStateM(qm, QState (vars_dom, qnprod))) = measure_vars i q Q" and
+   a1:"\<forall>e \<in> q. QStateM_map Q e \<noteq> {}" and a2:"q \<noteq> {}" and a4:"\<delta>k > 0" and
+   a3:"QStateM_vector Q \<noteq> 0\<^sub>v (2^(card (QStateM_vars Q)))"
+  shows "length (QStateM_list Q) = length qnprod"
+proof-  
+  have wf:"QState_wf (vars_dom,qnprod)" and wfm:"QStateM_wf (qm, QState(vars_dom,qnprod))"
+    using measure_vars_wf[OF a0 a1 a2 a4] by auto
+  then have "QStateM_map (QStateM(qm, QState (vars_dom, qnprod))) = QStateM_map Q"
+    using measure_vars_QStateM_map[OF a1 a2 a4 a0]
+    by auto
+  then have "QStateM_vars Q = QStateM_vars (QStateM(qm, QState (vars_dom, qnprod)))"
+    by (metis QStateM_wf eq_QStateM_vars fst_conv)
+  thus ?thesis 
+    using QStateM_wf_vars QState_rel1' QState_var_idem local.wf wfm
+    by (simp add: QStateM_list.rep_eq QStateM_vars.rep_eq)
+qed
+
+lemma  measure_vars'_eq_length_vector:
+  assumes
+   a0:"(\<delta>k, QStateM(qm, QState (vars_dom, qnprod))) = measure_vars' i q Q" and
+   a1:"\<forall>e \<in> q. QStateM_map Q e \<noteq> {}" and a2:"q \<noteq> {}" and a4:"\<delta>k > 0" and
+   a3:"QStateM_vector Q \<noteq> 0\<^sub>v (2^(card (QStateM_vars Q)))"
+  shows "length (QStateM_list Q) = length qnprod"
+proof-  
+  have wf:"QState_wf (vars_dom,qnprod)" and wfm:"QStateM_wf (qm, QState(vars_dom,qnprod))"
+    using measure_vars'_wf[OF a0 a1 a2 a4] by auto
+  then have "QStateM_map (QStateM(qm, QState (vars_dom, qnprod))) = QStateM_map Q"
+    using measure_vars'_QStateM_map[OF a1 a2 a4 a0]
+    by auto
+  then have "QStateM_vars Q = QStateM_vars (QStateM(qm, QState (vars_dom, qnprod)))"
+    by (metis QStateM_wf eq_QStateM_vars fst_conv)
+  thus ?thesis 
+    using QStateM_wf_vars QState_rel1' QState_var_idem local.wf wfm
+    by (simp add: QStateM_list.rep_eq QStateM_vars.rep_eq)
+qed
+
+lemma a_div_b_gt_0_b_not_zero:"(a::('a::linordered_field)) div b = \<sigma> \<Longrightarrow>  0 < \<sigma> \<Longrightarrow> b\<noteq>0"  
+  by force
+
+lemma a_div_b_gt_0_a_gt_zero:
+      assumes a0:"(a::('a::linordered_field)) div b = \<sigma>" and a1:"b\<ge>0" and a2:"\<sigma> > 0" 
+      shows "a > 0"
+  apply (cases "a=0")
+  using a0 a1 a2 divide_neg_pos  
+  by (auto simp add:zero_less_divide_iff)
+
+
+
+
+definition pr ::"'s expr_q  \<Rightarrow> ('s \<Rightarrow> complex list) \<Rightarrow> nat \<Rightarrow>  's state \<Rightarrow> real" 
+  where "pr q v i s \<equiv> let st = get_stack s ; qv = fst (get_qstate s); 
+                         vars = Q_domain qv; d1 = Q_domain_set q qv st; d2 = vars - d1 in 
+                     (\<Sum>j = 0..<2^(card d2). norm (aij s q v i j )^2) / 
+                        (\<Sum>i = 0 ..<2^(card d1). 
+                            \<Sum>j = 0 ..<2^(card d2). norm (aij s q v i j)^2 )"
+
+definition vector_i::"'s state \<Rightarrow> 's expr_q  \<Rightarrow>  ('s, complex list) expr \<Rightarrow> nat \<Rightarrow> ('s, complex list) expr"
+  where "vector_i s q v i \<equiv> 
+     let st = get_stack s ; qv = fst (get_qstate s); 
+               vars = Q_domain qv; d1 = Q_domain_set q qv st; d2 = vars - d1;
+        elem_ij  = (\<lambda>j. (aij s q v i j) / sqrt (pr q v i s)) in
+     (\<lambda>st. map (\<lambda>e. elem_ij e) [0..<2^card d2])"
+
+definition
+  unit_vecl :: "'s state \<Rightarrow> 's expr_q  \<Rightarrow> nat \<Rightarrow> ('s, complex list) expr"
+  where "unit_vecl s q i \<equiv>
+    let st = get_stack s ; qv = fst (get_qstate s); 
+        d1 = Q_domain_set q qv st in
+      (\<lambda>s. list_of_vec (unit_vec (2^card d1) i))"
+
+
+
+
+(*  " v \<in> nat_vars \<Longrightarrow>
+           not_access_v q v \<Longrightarrow>  not_access_v vl v \<Longrightarrow>                                             
+           \<turnstile> (q \<cdot> qr \<mapsto> vl)
+                (Measure v q)   
+              {s. s \<in> (\<Union>i\<in>{q}\<^sub>s. (v\<down>\<^sub>(from_nat i)) \<inter> ((q \<mapsto> (unit_vecl s q i)) \<and>\<^sup>* 
+                                  (qr  \<mapsto> (vector_i s q vl i)))\<smile>(\<rho> q vl i s))}" 
+*)
+(* lemma measure_vars_list:
+  assumes 
+     a0:"QStateM_vars Q = Q_domain_var (q \<union> qr) (QStateM_map Q)" and
+     a1:"QStateM_list Q = vl" and
+     a2:"QStateM_vars Q \<noteq> {}" and a3:"(\<forall>e\<in>q. QStateM_map Q e \<noteq> {})" and
+     a4:"q  \<inter> qr = {}" and
+     a5:"(p,Q') = measure_vars i q Q"
+   shows "QStateM_vector Q'  = Q
+             partial_state2.ptensor_vec (\<Union> (QStateM_map Q ` q)) 
+                                        (\<Union> (QStateM_map Q ` qr))  
+                                        (vec_of_list (unit_vecl (p,\<sigma>,Q) q i \<sigma>))
+                                        (vec_of_list (vector_i (p,\<sigma>,Q) q vl i \<sigma>))"
+proof-
+  have "a \<cdot>\<^sub>v ((ptensor_mat v1 v2 ((1\<^sub>k (2^(card v1)))) (1\<^sub>m (2^(card v2)))) *\<^sub>v v) = 
+            a \<cdot>\<^sub>v ptensor_vec v1 v2 (unit_vec (2^(card v1)) k) (vector_aij v1 v2 v k)"
+qed
+ *)
+
+
+(*lemma measure_vars_pr:
+  assumes 
+     a0:"QStateM_vars Q = Q_domain_var (q \<sigma> \<union> qr \<sigma>) (QStateM_map Q)" and
+     a1:"QStateM_list Q = vl \<sigma>" and
+     a2:"QStateM_vars Q \<noteq> {}" and a3:"(\<forall>e\<in>q \<sigma>. QStateM_map Q e \<noteq> {})" and
+     a4:"q \<sigma> \<inter> qr \<sigma> = {}" and
+     a5:"(p,Q') = measure_vars i (\<Union> (QStateM_map Q ` q \<sigma>)) Q"
+   shows "p = pr q vl i (pq,\<sigma>,Q')"
+  unfolding pr_def
+  sorry *)
+
 
 lemma allocate_wf1:
   assumes a0:"\<Q>' = QStateM(\<vv>', QState (q'_addr,(v \<sigma>)))" and  a1:"length (v \<sigma>) > 1" and     
@@ -423,8 +1552,8 @@ inductive QExec::"('v, 's) com \<Rightarrow> 's XQState \<Rightarrow> 's XQState
 
  | Dispose: "  \<Q> = \<Q>' + \<Q>'' \<Longrightarrow> \<Q>' ## \<Q>'' \<Longrightarrow> n = vec_norm (QStateM_vector \<Q>') \<Longrightarrow>
               QStateM_vars \<Q>' \<noteq> {} \<Longrightarrow> 
-              QStateM_vars \<Q>' = (Q_domain_var (var_set q i \<sigma>) (QStateM_map \<Q>')) \<Longrightarrow>                                      
-              \<forall>e \<in> (var_set q i \<sigma>). (QStateM_map \<Q>') e \<noteq> {} \<Longrightarrow>
+              QStateM_vars \<Q>' = (Q_domain_var (the (var_set q i \<sigma>)) (QStateM_map \<Q>')) \<Longrightarrow>                                      
+              \<forall>e \<in> (the (var_set q i \<sigma>)). (QStateM_map \<Q>') e \<noteq> {} \<Longrightarrow>
              \<turnstile> \<langle>Dispose q i, Normal (\<delta>,\<sigma>,\<Q>)\<rangle> \<Rightarrow> Normal (\<delta>,\<sigma>, n \<cdot>\<^sub>Q  \<Q>'')"
 
 \<comment>\<open>Dispose dispose will fail if it is not possible to find such states \<qq>',  \<qq>''\<close>
@@ -435,8 +1564,8 @@ inductive QExec::"('v, 's) com \<Rightarrow> 's XQState \<Rightarrow> 's XQState
                \<turnstile> \<langle>Dispose q, Normal (\<delta>,\<sigma>,\<Q>)\<rangle> \<Rightarrow> Fault" *)
 
 | Dispose_F: "\<nexists>\<Q>' \<Q>''.  \<Q> = \<Q>' + \<Q>'' \<and> \<Q>' ## \<Q>'' \<and> QStateM_vars \<Q>' \<noteq> {} \<and> 
-               QStateM_vars \<Q>' = (Q_domain_var (var_set q i \<sigma>) (QStateM_map \<Q>')) \<and>
-               (\<forall>e \<in> (var_set q i \<sigma>). (QStateM_map \<Q>') e \<noteq> {}) \<Longrightarrow>
+               QStateM_vars \<Q>' = (Q_domain_var (the (var_set q i \<sigma>)) (QStateM_map \<Q>')) \<and>
+               (\<forall>e \<in> (the (var_set q i \<sigma>)). (QStateM_map \<Q>') e \<noteq> {}) \<Longrightarrow>
                \<turnstile> \<langle>Dispose q i, Normal (\<delta>,\<sigma>,\<Q>)\<rangle> \<Rightarrow> Fault"
 
 \<comment>\<open>Measure measures the value of the set of qubits given by q \<sigma> and it stores the result in 
@@ -448,18 +1577,16 @@ inductive QExec::"('v, 's) com \<Rightarrow> 's XQState \<Rightarrow> 's XQState
             \<delta>k > 0 \<Longrightarrow> \<delta>' = \<delta> * \<delta>k \<Longrightarrow> \<sigma>' = set_value \<sigma> v (from_nat k) \<Longrightarrow>
             \<turnstile> \<langle>Measure v q, Normal (\<delta>,\<sigma>,(\<vv>,\<qq>))\<rangle> \<Rightarrow> Normal (\<delta>',\<sigma>',(\<vv>',\<qq>'))"  *)
 
-| Measure: "addr1 = \<Union>((QStateM_map \<Q>) ` (q \<sigma>)) \<Longrightarrow>
-            (QStateM_vars \<Q>) = addr1 \<union> addr2 \<Longrightarrow>            
-            k \<in> {0.. 2^(card addr1)} \<Longrightarrow>              
-            (\<delta>k, \<Q>') = measure_vars k addr1 \<Q> \<Longrightarrow>             
+| Measure: "addr1 = \<Union>((QStateM_map \<Q>) ` (q \<sigma>)) \<Longrightarrow> \<forall>e \<in> (q \<sigma>). (QStateM_map \<Q>) e \<noteq> {} \<Longrightarrow>                      
+            k \<in> {0..<2^(card addr1)} \<Longrightarrow>              
+            (\<delta>k, \<Q>') = measure_vars' k (q \<sigma>) \<Q> \<Longrightarrow>             
             \<delta>k > 0 \<Longrightarrow> \<delta>' = \<delta> * \<delta>k \<Longrightarrow> \<sigma>' = set_value \<sigma> v (from_nat k) \<Longrightarrow>
             \<turnstile> \<langle>Measure v q, Normal (\<delta>,\<sigma>,\<Q>)\<rangle> \<Rightarrow> Normal (\<delta>',\<sigma>',\<Q>')"
 \<comment>\<open>Since Measure access to the values of the qubits given by q \<sigma> as QMod, 
   Measure will similarly fail if the set of qubits to be mesured does not
   belong to the set of allocated qubits\<close>
 
- | Measure_F: "\<nexists>\<Q>' \<Q>''. \<not>(\<Union>((QStateM_map \<Q>') ` (q \<sigma>)) = (QStateM_vars \<Q>')) \<and>  
-               \<Q> = \<Q>' + \<Q>'' \<and> \<Q>' ## \<Q>'' \<Longrightarrow> 
+ | Measure_F: "\<exists>e. e \<in> q \<sigma> \<and> (QStateM_map \<Q>) e = {}  \<Longrightarrow> 
               \<turnstile> \<langle>Measure v q, Normal (\<delta>,\<sigma>,\<Q>)\<rangle> \<Rightarrow> Fault" 
 
 | Fault_Prop:"\<turnstile> \<langle>C, Fault\<rangle> \<Rightarrow> Fault"
